CertiGC/verif_resume.v
@@ -102,7 +102,9 @@ Proof.
       simpl fold_left.
       replace (WORD_SIZE * 0)%Z with 0 by lia.
       rewrite !isptr_offset_val_zero by assumption.
-      entailer!. rewrite H1. simpl tl.
+      rewrite H1. simpl tl.
+      rewrite Z.sub_0_r.
+      entailer_for_return.
       assert (MAX_SPACES = Zlength (map space_tri hl) + 1). {
         pose proof (spaces_size (ti_heap t_info)).
         rewrite <- H2, H1, Zlength_cons, Zlength_map. lia. } rewrite !H2.
